# Transformations
 
```{r, echo = F, out.width="80%", fig.cap="[Download Slides](slides/05-Transformations.pdf)"}
knitr::include_graphics("slides/gifs/05-Transformations.gif")
```

## Squared Terms in Regression Models

```{r}
# First Idea
summary(mod <- lm(dist ~ 1 + speed, data = cars))
plot(cars$speed,cars$dist)
abline(mod)
```


```{r}
# Introducing Transformations
df <- cars
df$speed_sq <- cars$speed^2
```

```{r}
# More Models
summary(mod2 <- lm(dist ~ 1 + speed_sq, data = df))
summary(mod3 <- lm(dist ~ 1 + speed + speed_sq, data = df))

plot(cars$speed,cars$dist)
model <- function(x){2.47 + 0.91 * x + 0.099 * x^2}
points(1:100, sapply(1:100, model), col="red",type="l")

model_sqonly <- function(x){8.86 + 0.129 * x^2}
points(1:100, sapply(1:100,model_sqonly), col="blue",type="l")
```


```{r}
# Removing Heteroscedasticity
summary(mod4 <- lm(log(dist) ~ 1 + speed + speed_sq, data = df))
summary(mod5 <- lm(log(dist) ~ -1 + speed + speed_sq, data = df))
summary(mod5 <- lm(log(dist) ~ -1  + speed_sq, data = df))
```


```{r}
# TODO: Add final plot
```



## Elasticity

> An elasticity coefficient is the ratio of the percentage change in the
> forecast variable ($y$) to the percentage change in the predictor
> variable ($x$). Mathematically, the elasticity is defined as
> $(dy/dx)\times(x/y)$. Consider the log-log model, $$
> \log y=\beta_0+\beta_1 \log x + \varepsilon.
> $$ Express $y$ as a function of $x$ and show that the coefficient
> $\beta_1$ is the elasticity coefficient.



$$ \log(y) = \beta_0 + \beta_1 \log(x) + \varepsilon \qquad \mid \mathbb{E}(\cdot \mid x)$$
Taking the conditional expectation on the left and right hand side of the quation

$$\mathbb{E}(\log(y) \mid x) = \mathbb{E}(\beta_0 + \beta_1 \log(x) + \varepsilon \mid x)$$
leads to the following as $\mathbb{E}(\varepsilon\mid x) = 0$.

$$ \log(y) = \beta_0 + \beta_1 \log(x) \qquad \mid \frac{\partial}{\partial x}$$
After taking derivatives of the left and right side with respect to $x$ we receive. The left hand side follows due to the implicit differentiation.

$$ \frac{\partial}{\partial x}\log(y) = \frac{\partial}{\partial x}(\beta_0 + \beta_1 \log(x))$$



$$\frac{\partial\log(y)}{\partial x} = 0 + \beta_1 \frac{1}{x}$$
$$\frac{1}{y} \frac{\partial y}{\partial x} = \beta_1 \frac{1}{x} \qquad \mid \cdot x$$

After rearranging we get the definition of the the elasticity.

$$\beta_1 = \frac{x}{y} \frac{\partial y}{\partial x}$$

